AbstractStore.v
@@ -1,0 +1,19 @@
+Require Import Maps.
+Require Import Parity.
+
+Definition store := total_map nat.
+Definition abstract_store := total_map parity.
+
+Definition sound_store (ast : abstract_store) (st : store) : Prop := 
+  forall x, gamma_par (ast x) (st x).
+
+Lemma t_update_sound : forall ast st x p n,
+  sound_store ast st ->
+  sound_par p n ->
+  sound_store (t_update ast x p) (t_update st x n).
+Proof. 
+  intros. unfold sound_store.  intros. unfold t_update. 
+  destruct (beq_string x x0). 
+  - unfold sound_par in H0. assumption.
+  - unfold sound_store in H. apply H.
+Qed.
